KmsArnIdentifier.dfy
@@ -1,0 +1,79 @@
+predicate ArnString?(s: string)
+{
+    s == "arn"
+}
+// MUST start with string arn
+type ArnString = s:string | ArnString?(s) witness *
+
+// The partition MUST be a non-empty
+type PartitionString = s:string | |s| != 0 witness "a"
+
+// The service MUST be the string kms
+type ServiceString = s | s =="kms"
+
+// The region MUST be a non-empty string
+type RegionString = s:string | |s| != 0
+
+//The account MUST be a non-empty string
+type AccountString = s:string | |s| != 0
+
+
+// The resource section MUST be non-empty and MUST be split by a single / any additional / are included in the resource id
+// The resource type MUST be either alias or key
+// The resource id MUST be a non-empty string 
+// this seq<string> length is 2, x[0] is key, x[1] is ID.
+
+type KmsResourceSeqStr = x:seq<string> | |x| == 2 && (x[0]=="alias" || x[0] == "key") && |x[1]| != 0
+
+datatype ARN = ARN(
+    arnLiteral: string,
+    partition: string,
+    service: string,
+    region: string,
+    account: string,
+    resource: seq<string>
+)
+
+
+
+type KmsArn = a: ARN | KmsArn?(a)
+
+
+predicate KmsArn?(a:ARN)
+{
+    if
+        // MUST start with string arn
+        && a.arnLiteral == "arn"
+
+        // The partition MUST be a non-empty
+        && |a.partition| !=0
+
+        // The service MUST be the string kms
+        && a.service == "kms"
+
+        //The account MUST be a non-empty string
+        && |a.account| != 0
+
+        // The region MUST be a non-empty string
+        && |a.region| !=0
+
+        // then it leads to resource type to be key or alias, and both id cannot be empty
+        &&  (
+            (&& a.resource[0] == "key"
+            && |a.resource[1]|!=0 ) 
+            || 
+            (&& a.resource[0] == "alias" 
+            && |a.resource[1]| != 0 )
+            )
+    then true
+    else false
+}
+
+method test()
+{
+    assert ARN("arn","aws","kms","us-east-1","2222222222222",["key","testid"]).ARN?;
+
+
+    assert KmsArn?(ARN("arn","aws","kms","us-east-1","2222222222222",["key","testid"])) == true;
+
+}
